Proven soundness of dispose. QState is constrain to allow only complex numbers with the real part strictly greater than zero and the imaginary part equal to 0. This is necessary to prove soundness of the dispose operation.

QSyntax.thy
@@ -31,9 +31,9 @@ of the different variables, the vector dimension is the product of the size of e
 variable\<close> 
 
 type_synonym q_vars = "(nat \<Rightarrow>nat set)"
-type_synonym qstate = "q_vars \<times> (complex) QState"
+type_synonym qstate = "q_vars \<times>  QState"
 type_synonym qheap = "nat set \<times> complex vec"
-type_synonym 's state = "real \<times> 's \<times>  (complex) QStateM"
+type_synonym 's state = "real \<times> 's \<times>   QStateM"
 type_synonym 's pred = "'s \<Rightarrow> bool" 
 type_synonym 's assn = "'s set"
 type_synonym 's expr_q = "'s \<Rightarrow> nat set"
@@ -46,7 +46,7 @@ type_synonym ('s,'b) expr = "'s \<Rightarrow> 'b"
 definition get_prob ::"'s state \<Rightarrow> real"
   where "get_prob \<sigma> \<equiv> fst \<sigma>"
 
-definition get_QStateM ::"'s state \<Rightarrow> complex QStateM"
+definition get_QStateM ::"'s state \<Rightarrow>  QStateM"
   where "get_QStateM \<sigma> \<equiv> snd (snd \<sigma>)"
 
 definition get_qstate ::"'s state \<Rightarrow> qstate"
@@ -58,7 +58,7 @@ definition get_stack::"'s state \<Rightarrow> 's"
 definition set_prob ::"'s state \<Rightarrow> real \<Rightarrow> 's state"
   where "set_prob \<sigma> v = (v, get_stack \<sigma>, get_QStateM \<sigma>)"
 
-definition set_qstate ::"'s state \<Rightarrow>  complex QStateM \<Rightarrow> 's state"
+definition set_qstate ::"'s state \<Rightarrow>   QStateM \<Rightarrow> 's state"
   where "set_qstate \<sigma> v = (get_prob \<sigma>, get_stack \<sigma>,  v)"
 
 definition set_stack::"'s state \<Rightarrow> 's \<Rightarrow> 's state"
@@ -155,7 +155,7 @@ definition lin_sets::"'q::linorder set \<Rightarrow> 'q::linorder set \<Rightarr
 definition sorted_list_from_set::"'q::linorder set \<Rightarrow> 'q::linorder list"
   where "sorted_list_from_set s \<equiv> THE l. strict_sorted l \<and> set l = s"
 
-definition to_heap::"qstate \<Rightarrow> (complex) QState"
+definition to_heap::"qstate \<Rightarrow>  QState"
   where "to_heap q \<equiv> (snd q)"
 
 
