Q_State.thy
@@ -262,7 +262,7 @@ typedef
 
 setup_lifting type_definition_QState
 
-definition tensor_mat_ord::"'a QState \<Rightarrow> nat set \<Rightarrow> 'a::comm_ring_1 mat \<Rightarrow> 'a QState set"
+definition tensor_mat_ord::"QState \<Rightarrow> nat set \<Rightarrow> complex mat \<Rightarrow> QState set"
   where "tensor_mat_ord Q q M \<equiv> {}"
 
 lemma QState_rel1:"length(snd(uQState x)) = 2 ^ card (fst(uQState x))"
@@ -272,31 +272,31 @@ lemma QState_rel1:"length(snd(uQState x)) = 2 ^ card (fst(uQState x))"
                   (((snd (uQState x)) ! 0) = 1)"
   by (transfer, auto) *)
 
-lemma QState_rel2:"length(snd(uQState x)) =  0 \<longrightarrow>
-                   (snd (uQState x)) \<noteq> [0]"
+lemma QState_rel2:"length(snd(uQState x)) =  1 \<longrightarrow>
+                   Im (snd (uQState x) ! 0) = 0 \<and> Re (snd (uQState x) ! 0) > 0"
   apply transfer by auto
 
 
-lemma QState_rel3:"finite (fst (uQState (x::('a::field) QState )))"
+lemma QState_rel3:"finite (fst (uQState (x:: QState )))"
   apply transfer by auto
 
 
 
-lift_definition QState_vars :: "('a::field) QState \<Rightarrow> nat set" is fst .
-lift_definition QState_list :: "('a::field) QState \<Rightarrow> 'a list" is snd .
-lift_definition QState_vector::"('a::field) QState \<Rightarrow> 'a vec" is "\<lambda>s. vec_of_list (snd s)" .
+lift_definition QState_vars :: "QState \<Rightarrow> nat set" is fst .
+lift_definition QState_list :: "QState \<Rightarrow> complex list" is snd .
+lift_definition QState_vector::"QState \<Rightarrow> complex vec" is "\<lambda>s. vec_of_list (snd s)" .
 
-abbreviation QState_wf::"nat set \<times> 'a::field list \<Rightarrow> bool"
+abbreviation QState_wf::"nat set \<times> complex list \<Rightarrow> bool"
   where "QState_wf s \<equiv> 
       length (snd s) = (2^(card (fst s))) \<and> 
       finite (fst s) \<and> 
-      (length (snd s) = 1 \<longrightarrow> (snd s)\<noteq>[0])"
+      (length (snd s) = 1 \<longrightarrow> Im ((snd s)!0) = 0 \<and> Re ((snd s)!0) > 0)"
 
-lift_definition QState :: "nat set \<times> 'a::field list \<Rightarrow> 'a QState" is  
+lift_definition QState :: "nat set \<times> complex list \<Rightarrow> QState" is  
   "\<lambda>s. if QState_wf s then (fst s, snd s)
        else ({}, [1])"  by auto
 
-abbreviation QState_unfold ::"'a::field QState \<Rightarrow> nat set \<times> 'a::field list"
+abbreviation QState_unfold ::"QState \<Rightarrow> nat set \<times> complex list"
   where "QState_unfold x \<equiv> (QState_vars x, QState_list x)"
 
 lemma QState_wf:"QState_wf (QState_unfold x)"
@@ -310,33 +310,31 @@ lemma QState_list_idem:"QState_wf (vs, v) \<Longrightarrow>
        QState_list (QState (vs, v)) = v"
   by (transfer, auto)
 
-lift_definition Conc :: " 'a QState \<Rightarrow> nat set \<times> 'a::field vec" is
+lift_definition Conc :: " QState \<Rightarrow> nat set \<times> complex vec" is
   "\<lambda>s. (QState_vars s, QState_vector s)" .
 
-definition sca_mult_qstate::"'a::field \<Rightarrow> 'a QState \<Rightarrow> 'a QState"  (infixl "\<cdot>\<^sub>q" 70) 
+definition sca_mult_qstate::"complex \<Rightarrow>  QState \<Rightarrow>  QState"  (infixl "\<cdot>\<^sub>q" 70) 
   where "sca_mult_qstate s qs \<equiv> QState(QState_vars qs, list_of_vec (s \<cdot>\<^sub>v (QState_vector qs)))"
 
 lemma sca_mult_qstate_wf:
-  assumes a0:"(s::'a::field) \<noteq> 0" 
+  assumes a0:"Im s = 0 \<and> Re (s::complex) > 0" 
   shows "QState_wf (QState_vars qs, list_of_vec (s \<cdot>\<^sub>v (QState_vector qs)))"  
 proof-
   have wf:"QState_wf (QState_unfold qs)"
     using QState_wf by blast
   
   { assume "length (QState_list qs) = 1"    
-    then obtain v where v:"QState_list qs = [v] \<and> v \<noteq> 0"
+    then obtain v where v:"QState_list qs = [v] \<and> Im v = 0 \<and> Re v > 0"
       using wf
-      by (metis One_nat_def Suc_length_conv length_0_conv snd_conv) 
-    then have "s * v \<noteq> 0" using a0 by auto
+      by (metis One_nat_def Suc_length_conv list_exhaust_size_eq0 nth_Cons_0 sndI)
+    then have f1:"Im (s * v) = 0 \<and> Re (s * v) > 0" using a0 by auto
     then have ?thesis using v
     proof -
       have "snd (uQState qs) = [v]"
         by (metis (no_types) QState_list.rep_eq v)
-      then show ?thesis
-        by (metis (no_types) QState_rel1 QState_rel3 QState_vars.rep_eq 
-            QState_vector.rep_eq \<open>s * v \<noteq> 0\<close> dim_vec_of_list fst_conv 
-            index_smult_vec(1) index_smult_vec(2) neq0_conv snd_conv 
-            vec_index_vCons_0 vec_list vec_of_list_Cons zero_neq_one)
+      then show ?thesis        
+        using  f1 local.wf v apply transfer by auto
+
     qed                                             
   }
   moreover { 
@@ -349,30 +347,31 @@ proof-
   ultimately show ?thesis by auto
 qed
 
-lemma sca_mult_qstate_vars:"(s::'a::field) \<noteq>0 \<Longrightarrow>QState_vars (s \<cdot>\<^sub>q qs) = QState_vars qs"
+lemma sca_mult_qstate_vars:"Im s = 0 \<and> Re (s::complex) > 0 \<Longrightarrow>QState_vars (s \<cdot>\<^sub>q qs) = QState_vars qs"
   unfolding sca_mult_qstate_def using sca_mult_qstate_wf
   using QState_var_idem by blast
 
 lemma sca_mult_qstate_quantum: 
-  "(s::'a::field) \<noteq>0 \<Longrightarrow> QState_vector (s \<cdot>\<^sub>q qs) = s \<cdot>\<^sub>v (QState_vector qs)"
+  "Im s = 0 \<and> Re (s::complex) > 0 \<Longrightarrow> QState_vector (s \<cdot>\<^sub>q qs) = s \<cdot>\<^sub>v (QState_vector qs)"
   unfolding sca_mult_qstate_def using sca_mult_qstate_wf[of s qs]  
   apply transfer 
   by (simp add: vec_list)
 
 lemma sca_mult_qstate_assoc: 
-  "a1 \<noteq> 0 \<Longrightarrow> a2\<noteq>0 \<Longrightarrow> (a1::'a::field)* a2 \<cdot>\<^sub>q qs = a1 \<cdot>\<^sub>q (a2 \<cdot>\<^sub>q qs)" 
+  "Im a1 = 0 \<and> Re a1 > 0 \<Longrightarrow> Im a2 = 0 \<and> Re a2 > 0 \<Longrightarrow> 
+   a1 * a2 \<cdot>\<^sub>q qs = a1 \<cdot>\<^sub>q (a2 \<cdot>\<^sub>q qs)" 
   by (metis (no_types) sca_mult_qstate_def 
     sca_mult_qstate_quantum sca_mult_qstate_vars smult_smult_assoc)
 
   
-definition empty_qstate::"'a::field QState"  ("|>") 
+definition empty_qstate::"QState"  ("|>") 
   where "empty_qstate  \<equiv> QState({}, [1])"
 
 
 lemma uqstate_fst:"fst (uQState a) = QState_vars a" apply transfer' by auto
 lemma uqstate_snd:"snd (uQState a) = QState_list a" apply transfer' by auto
 
-lemma QState_rel3':"finite (QState_vars (x::('a::field) QState ))"
+lemma QState_rel3':"finite (QState_vars (x:: QState ))"
   by (transfer, auto)
 
 lemma QState_rel1':"length(QState_list x) = 2 ^ card (QState_vars x)"
@@ -449,17 +448,20 @@ lemma QState_list_inv: assumes a0:"QState_vars Q = {}"
   shows "inverse(QState_list Q ! 0) \<cdot>\<^sub>q Q = |>"
   unfolding empty_qstate_def sca_mult_qstate_def using a0 apply transfer' 
   apply auto
-  by (simp add: list_of_vec_map vec_of_list_index)
-  
+  subgoal for b
+    apply (subgoal_tac "b ! 0 \<noteq> 0")
+     apply (auto simp add: list_of_vec_map vec_of_list_index)
+    done
+  done
 
-definition plus_QState_vector::"('a::field) QState \<Rightarrow> 'a QState \<Rightarrow>nat set \<times> 'a list"
+definition plus_QState_vector::"QState \<Rightarrow>  QState \<Rightarrow>nat set \<times> complex list"
   where "plus_QState_vector q1 q2 \<equiv> 
      let d1 = QState_vars q1; 
          d2 = QState_vars q2; 
          l1 = QState_vector q1; l2 = QState_vector q2 in
           (d1 \<union> d2, list_of_vec(partial_state2.ptensor_vec d1 d2 l1 l2))"
 
-definition vector_element_12::"('a::field) QState \<Rightarrow> nat set \<Rightarrow> nat \<times> nat \<Rightarrow> 'a"
+definition vector_element_12::"QState \<Rightarrow> nat set \<Rightarrow> nat \<times> nat \<Rightarrow> complex"
   where "vector_element_12 v d1 p \<equiv> 
          let d = QState_vars v; 
          d2 = d - d1; 
@@ -481,7 +483,7 @@ lemma QState_vars_empty:"QState_vars (QState ({}, [1])) = {}"
 lemma plus_QState_vector_a_idem:
   "snd (plus_QState_vector a (QState ({}, [1]))) = QState_list a"  
 proof-
-  let ?v0 = "QState ({}, [1])::('a) QState"  
+  let ?v0 = "QState ({}, [1]):: QState"  
   let ?v = "(QState_vars a)"
   let ?v1 = "{}"
   let ?s = "list_dims ?v"
@@ -500,13 +502,13 @@ proof-
      using  v1  apply transfer' by (auto simp add: list_vec)          
 qed
 
-definition plus_QState:: "('a::field) QState \<Rightarrow> 'a QState \<Rightarrow> 'a QState"
+definition plus_QState:: "QState \<Rightarrow>  QState \<Rightarrow> QState"
   where "plus_QState q1 q2 \<equiv> 
     let d1 = (QState_vars q1); d2 = (QState_vars q2) in
       if (d1 \<inter> d2 \<noteq> {}) then QState ({},[1])
       else QState (plus_QState_vector q1 q2)"
 
-definition disj_QState::"('a::field) QState \<Rightarrow> 'a QState \<Rightarrow> bool"
+definition disj_QState::"QState \<Rightarrow>  QState \<Rightarrow> bool"
   where "disj_QState q1 q2 \<equiv> QState_vars q1 \<inter> QState_vars q2 = {}"
 
 \<comment>\<open>Lemmas on plus_QState_vector\<close>
@@ -592,22 +594,27 @@ lemma plus_QState_vector_wf: assumes a0: "QState_vars q1 \<inter> QState_vars q2
 lemma plus_QState_vector_wf_empty:
   assumes a0:"QState_vars q1 \<inter> QState_vars q2 = {}" and
           a1:"fst (plus_QState_vector q1 q2) = {}"
-        shows "snd (plus_QState_vector q1 q2) \<noteq> [0]"
+        shows "Im ((snd (plus_QState_vector q1 q2)) ! 0) = 0 \<and>
+               Re ((snd (plus_QState_vector q1 q2)) ! 0) > 0"
 proof-
+  let ?pt = "(ptensor_vec (QState_vars q1) (QState_vars q2) (QState_vector q1) (QState_vector q2))"
   have "QState_vars q1 = {}" and "QState_vars q2 = {}"
     using a1 unfolding plus_QState_vector_def Let_def by auto  
-  moreover have "QState_vector q1 $ 0 \<noteq> 0" and "QState_vector q2 $ 0 \<noteq> 0"
+  moreover have "Im (QState_vector q1 $ 0) =0 \<and> Re (QState_vector q1 $ 0) > 0" and 
+                "Im (QState_vector q2 $ 0) = 0 \<and> Re (QState_vector q2 $ 0) > 0"
     using calculation apply auto apply transfer
-     apply (metis One_nat_def Suc_length_conv card_empty fstI 
-              list_exhaust_size_eq0 nth_Cons_0 power_0 sndI vec_of_list_index)
+     apply (metis card_empty class_semiring.nat_pow_0 fst_conv snd_conv vec_of_list_index )
+      apply transfer
+     apply (metis card_empty class_semiring.nat_pow_0 fst_conv snd_conv vec_of_list_index )
     apply transfer
-    by (metis One_nat_def Suc_length_conv card_empty fstI 
-              list_exhaust_size_eq0 nth_Cons_0 power_0 sndI vec_of_list_index)
-  ultimately have "(ptensor_vec (QState_vars q1) (QState_vars q2) (QState_vector q1)
-            (QState_vector q2)) $ 0 \<noteq> 0" 
-    using ptensor_empty[of "QState_vector q1" "QState_vector q2"] by simp
-  then show ?thesis unfolding plus_QState_vector_def Let_def
-    by (metis nth_Cons_0 snd_conv vec_list vec_of_list_index)                                                     
+    apply (metis card_empty class_semiring.nat_pow_0 fst_conv snd_conv vec_of_list_index )   
+    apply transfer
+    by (metis card_empty class_semiring.nat_pow_0 fst_conv snd_conv vec_of_list_index )  
+  ultimately have "Im (?pt$0) = 0 \<and> Re (?pt$0) > 0" 
+    using ptensor_empty[of "QState_vector q1" "QState_vector q2"] 
+    by simp
+  then show ?thesis unfolding plus_QState_vector_def Let_def 
+    by (metis snd_conv vec_list vec_of_list_index)                                                     
 qed
 
 (* lemma plus_QState_vector_empty_vars_one_wf:
@@ -811,7 +818,7 @@ proof-
 qed
 
 
-instantiation QState :: (field) sep_algebra
+instantiation QState ::  sep_algebra
 begin
 definition zero_QState: "0 \<equiv> QState ({},[1])"
 definition plus_QState: "s1 + s2 \<equiv> plus_QState s1 s2" 
@@ -830,7 +837,7 @@ instance
 end 
 
 lemma scalar_mult_QState_plus_l:
-  assumes a0: "(a::'a::field) \<noteq> 0" and 
+  assumes a0: "Im a = 0 \<and> Re a > 0" and 
           a1:"Q' ## Q''"
         shows "a  \<cdot>\<^sub>q (Q' + Q'') = (a  \<cdot>\<^sub>q Q' + Q'')"
 proof-
@@ -863,7 +870,7 @@ proof-
 qed
 
 lemma scalar_mult_QState_plus_r: 
-  assumes a0: "(a::'a::field) \<noteq> 0" and 
+  assumes a0: "Im a = 0 \<and> Re a > 0" and 
           a1:"Q' ## Q''" 
   shows "a  \<cdot>\<^sub>q (Q' + Q'') = ( Q' + a  \<cdot>\<^sub>q Q'')"
 proof-
@@ -897,7 +904,7 @@ qed
 
 
 type_synonym q_vars = "(nat \<Rightarrow>nat set)"
-type_synonym  'a qstate = "q_vars \<times> 'a QState"
+type_synonym qstate = "q_vars \<times>  QState"
 
 definition Q_domain::"q_vars \<Rightarrow> nat set" 
   where "Q_domain q_vars \<equiv> \<Union> (range q_vars)"
@@ -906,13 +913,13 @@ definition ket_dim ::"q_vars \<Rightarrow> nat"
   where "ket_dim q_vars \<equiv>  card (Q_domain q_vars)"
 
 \<comment>\<open>\<close>
-abbreviation QStateM_wf::"q_vars \<times> ('a::field QState) \<Rightarrow> bool"
+abbreviation QStateM_wf::"q_vars \<times>  QState \<Rightarrow> bool"
   where "QStateM_wf s \<equiv> 
         Q_domain (fst s) = QState_vars (snd s) \<and>
         (\<forall>x y. x\<noteq>y \<and> x\<in> domain (fst s) \<and> y \<in> domain (fst s) \<longrightarrow> (fst s) x \<inter> (fst s) y = {})"
 
-typedef (overloaded) ('a::field)
-  QStateM = "{(m,q)| (m::q_vars) (q:: 'a QState). QStateM_wf (m,q)}"
+typedef 
+  QStateM = "{(m,q)| (m::q_vars) (q:: QState). QStateM_wf (m,q)}"
   morphisms uQStateM Abs_QStateM              
   unfolding Q_domain_def  apply auto apply transfer
   apply (rule exI[where x ="\<lambda>x. {}"], auto)
@@ -920,24 +927,24 @@ typedef (overloaded) ('a::field)
 
 setup_lifting type_definition_QStateM
 
-lift_definition QStateM_map :: "('a::field) QStateM \<Rightarrow> q_vars" is fst .
+lift_definition QStateM_map :: "QStateM \<Rightarrow> q_vars" is fst .
 
 abbreviation empty_map::"q_vars" ("{}\<^sub>q")
   where "empty_map \<equiv> (\<lambda>n. {})"
 
-definition qstate :: "('a::field) QStateM \<Rightarrow> 'a QState" 
+definition qstate :: "QStateM \<Rightarrow> QState" 
   where "qstate s \<equiv> snd (uQStateM s)"
 
-lift_definition QStateM_vars::"('a::field) QStateM \<Rightarrow> nat set" is "(\<lambda>s. QState_vars (snd s))" .
-lift_definition QStateM_list::"('a::field) QStateM \<Rightarrow> 'a list" is "(\<lambda>s. QState_list (snd s))" .
-lift_definition QStateM_vector::"('a::field) QStateM \<Rightarrow> 'a vec" is "(\<lambda>s. QState_vector (snd s))" .
+lift_definition QStateM_vars::"QStateM \<Rightarrow> nat set" is "(\<lambda>s. QState_vars (snd s))" .
+lift_definition QStateM_list::"QStateM \<Rightarrow> complex list" is "(\<lambda>s. QState_list (snd s))" .
+lift_definition QStateM_vector::" QStateM \<Rightarrow> complex vec" is "(\<lambda>s. QState_vector (snd s))" .
 
-lift_definition QStateM ::"q_vars \<times> ('a::field QState) \<Rightarrow> 'a QStateM" is
+lift_definition QStateM ::"q_vars \<times>  QState \<Rightarrow> QStateM" is
 "\<lambda>s. if QStateM_wf s then (fst s, snd s) else (\<lambda>s. {}, QState ({},[1]))"
   unfolding Q_domain_def by (auto simp add:  QState_vars_empty)
 
 
-abbreviation QStateM_unfold::"('a::field) QStateM \<Rightarrow> (q_vars \<times> 'a QState)"
+abbreviation QStateM_unfold::"QStateM \<Rightarrow> (q_vars \<times>  QState)"
   where "QStateM_unfold q \<equiv> (QStateM_map q, qstate q)"
 
 lemma eq_QStateM_vars:"QState_vars (snd (QStateM_unfold q)) = QStateM_vars q"
@@ -1015,11 +1022,11 @@ lemma a1:"\<Union> (range (0::nat \<Rightarrow> nat set)) = none"
 lemma a2:"QState_vars 0 = 0"
   by (simp add: QState_vars_empty zero_QState zero_set_def)
 
-definition sca_mult_qstatem::"'a::field \<Rightarrow> 'a QStateM \<Rightarrow> 'a QStateM"  (infixl "\<cdot>\<^sub>Q" 70)
+definition sca_mult_qstatem::"complex \<Rightarrow>  QStateM \<Rightarrow> QStateM"  (infixl "\<cdot>\<^sub>Q" 70)
   where "sca_mult_qstatem s qs \<equiv> QStateM(QStateM_map qs, s \<cdot>\<^sub>q (qstate qs))"
 
 lemma sca_mult_qstatem_wf:
-  assumes a0:"(s::'a::field) \<noteq> 0" shows "QStateM_wf (QStateM_map qs, s \<cdot>\<^sub>q (qstate qs))"
+  assumes a0:"Im s = 0 \<and> Re s > 0" shows "QStateM_wf (QStateM_map qs, s \<cdot>\<^sub>q (qstate qs))"
 proof-
   have "QStateM_wf (QStateM_unfold qs)"
     using QStateM_wf by blast
@@ -1028,12 +1035,12 @@ proof-
 qed
 
 lemma sca_mult_qstatem_var_map:
-  "(s::'a::field) \<noteq> 0 \<Longrightarrow> QStateM_map (s \<cdot>\<^sub>Q qs) = QStateM_map qs"
+  "Im s = 0 \<and> Re s > 0  \<Longrightarrow> QStateM_map (s \<cdot>\<^sub>Q qs) = QStateM_map qs"
   unfolding sca_mult_qstatem_def using sca_mult_qstatem_wf[of s qs]
   by (auto simp add: QStateM_wf_map)
 
 lemma sca_mult_qstatem_var_qstate:
-  "(s::'a::field) \<noteq> 0 \<Longrightarrow> qstate (s \<cdot>\<^sub>Q qs) = s \<cdot>\<^sub>q qstate qs"
+  "Im s = 0 \<and> Re s > 0 \<Longrightarrow> qstate (s \<cdot>\<^sub>Q qs) = s \<cdot>\<^sub>q qstate qs"
   unfolding sca_mult_qstatem_def using sca_mult_qstatem_wf[of s qs]
   by (auto simp add: QStateM_wf_qstate)
 
@@ -1051,19 +1058,18 @@ proof-
 qed
 
 lemma sca_mult_qstatem_assoc: 
-  "a1 \<noteq> 0 \<Longrightarrow> a2\<noteq>0 \<Longrightarrow> (a1::'a::field)* a2 \<cdot>\<^sub>Q Q = a1 \<cdot>\<^sub>Q (a2 \<cdot>\<^sub>Q Q)"
+  "Im a1 = 0 \<and> Re a1 > 0 \<Longrightarrow> Im a2 = 0 \<and> Re a2 > 0 \<Longrightarrow> a1 * a2 \<cdot>\<^sub>Q Q = a1 \<cdot>\<^sub>Q (a2 \<cdot>\<^sub>Q Q)"
   by (metis (no_types) sca_mult_qstate_assoc sca_mult_qstatem_def sca_mult_qstatem_var_map sca_mult_qstatem_var_qstate)
 
 
 lemma QStateM_empty_not_zero: assumes a0:"Q_domain (QStateM_map \<Q>) = {}"
-  shows "(QStateM_list \<Q> ! 0) \<noteq> 0"
+  shows "Im (QStateM_list \<Q> ! 0) = 0 \<and> Re (QStateM_list \<Q> ! 0) > 0"
 proof-
   have "QStateM_map \<Q> = {}\<^sub>q" using a0 unfolding Q_domain_def by auto       
   then have "QStateM_list \<Q> = QState_list (qstate \<Q>)"
     unfolding qstate_def apply transfer by auto  
   then show ?thesis apply auto unfolding qstate_def
-    by (metis One_nat_def QStateM_rel1 QState_list_empty QState_wf assms 
-        length_Cons list.size(3) nth_Cons_0 qstate_def snd_conv)
+    using QStateM_rel1 QState_wf assms qstate_def by auto
 qed
 
 lemma disjoint_x_y_wf1_x_plus_y:
@@ -1131,7 +1137,7 @@ lemma plus_wf: assumes a0:"QStateM_map x ## QStateM_map y "  and
   apply transfer' apply auto 
   sorry *)
 
-instantiation QStateM :: (field) sep_algebra
+instantiation QStateM ::  sep_algebra
 begin
 definition zero_QStateM: "0 \<equiv> QStateM (0, 0)"
 definition plus_QStateM: "s1 + s2 \<equiv> QStateM (QStateM_map s1 + QStateM_map s2, qstate s1 + qstate s2)" 
@@ -1143,8 +1149,8 @@ lemma h:"QStateM_map x + QStateM_map 0 = QStateM_map x"
 
 lemma qstate_idem:"qstate x + qstate 0 = qstate x"    
 proof -
-  have "uQStateM (0::'a QStateM) = (0, 0) \<or> 
-       snd (uQStateM (0::'a QStateM)) = 0"
+  have "uQStateM (0::QStateM) = (0, 0) \<or> 
+       snd (uQStateM (0::QStateM)) = 0"
     by (simp add: QStateM.rep_eq zero_QState zero_QStateM)
   then show ?thesis unfolding qstate_def
     by fastforce
@@ -1169,24 +1175,123 @@ instance
 end 
 
 lemma scalar_mult_QStateM_plus_l:
-  "(a::'a::field) \<noteq> 0 \<Longrightarrow> \<Q>' ## \<Q>'' \<Longrightarrow> a  \<cdot>\<^sub>Q (\<Q>' + \<Q>'') = (a  \<cdot>\<^sub>Q \<Q>' + \<Q>'')"
+  "Im a = 0 \<and> Re a > 0  \<Longrightarrow> \<Q>' ## \<Q>'' \<Longrightarrow> a  \<cdot>\<^sub>Q (\<Q>' + \<Q>'') = (a  \<cdot>\<^sub>Q \<Q>' + \<Q>'')"
   unfolding sca_mult_qstatem_def plus_QStateM sep_disj_QStateM
-  by (smt QStateM_wf_map QStateM_wf_qstate plus_wf sca_mult_qstatem_wf 
-          scalar_mult_QState_plus_l)
+  using QStateM_rel1 QStateM_rel2 QStateM_wf_map QStateM_wf_qstate plus_wf 
+         sca_mult_qstate_vars scalar_mult_QState_plus_l by auto
   
 
 lemma scalar_mult_QStateM_plus_r:
-  assumes a0:"(a::'a::field) \<noteq> 0" and a1:"\<Q>' ## \<Q>''" 
+  assumes a0:"Im a = 0 \<and> Re a > 0" and a1:"\<Q>' ## \<Q>''" 
   shows "a  \<cdot>\<^sub>Q (\<Q>' + \<Q>'') = ( \<Q>' + a  \<cdot>\<^sub>Q \<Q>'')"
-  by (smt a0 assms(2) plus_QStateM sca_mult_qstatem_def sca_mult_qstatem_var_map 
-       sca_mult_qstatem_var_qstate scalar_mult_QStateM_plus_l 
-         scalar_mult_QState_plus_l scalar_mult_QState_plus_r sep_disj_QStateM)
+  using a0 local.a1 plus_QStateM sca_mult_qstatem_var_map 
+        sca_mult_qstatem_var_qstate scalar_mult_QStateM_plus_l 
+        scalar_mult_QState_plus_l scalar_mult_QState_plus_r 
+        sep_disj_QStateM by auto
 
-lemma "vec_norm( u \<cdot>\<^sub>v v) = \<bar>u\<bar> * vec_norm v"
-  sorry
-lemma 
-  "vec_norm (QStateM_vector (QStateM_list \<Q>'' ! 0 \<cdot>\<^sub>Q \<Q>')) \<cdot>\<^sub>Q
+value "(5::nat) * ((vec_of_list[3,1,3])\<bullet>(vec_of_list[3,1,3]))"
+value " (((5::nat)\<cdot>\<^sub>v(vec_of_list[3,1,3]))\<bullet>(vec_of_list[3,1,3]))"
+value "((vec_of_list[3::nat,1,3,4])\<bullet>(vec_of_list[3,1,3]))"
+
+lemma "v \<in> carrier_vec n \<Longrightarrow> 
+       w \<in> carrier_vec n \<Longrightarrow> 
+       a * (v \<bullet> w) = (a \<cdot>\<^sub>v v) \<bullet> w"
+  by auto
+
+
+thm complex_norm_square
+lemma "\<bar>u::complex\<bar> = norm u"
+  by (simp add: abs_complex_def  of_real_def)
+
+ 
+lemma "(conjugate u::complex)\<cdot>\<^sub>v(conjugate v) = conjugate (u \<cdot>\<^sub>v v) "
+  by auto
+
+lemma Re_norm_v_gt_0:assumes a0:"Re u > 0 " and a1:"Re v > 0"
+  shows "Re (\<bar>u\<bar> * v) > 0" using a0 a1
+  proof -
+    have f1: "\<And>c. complex_of_real (cmod c) = \<bar>c\<bar>"
+      by (simp add: abs_complex_def)
+    then have f2: "\<And>c. Im \<bar>c\<bar> = 0"
+      by (metis (no_types) Im_complex_of_real)
+    have f3: "\<And>c. Re \<bar>c\<bar> = cmod c"
+      using f1 by (metis (no_types) Re_complex_of_real)
+    have "0 \<noteq> u"
+      using a0 by force
+    then show ?thesis
+      using f3 f2 by (simp add: a1)
+  qed
+
+lemma Re_norm_u_gt_0_Im_v_0:
+  assumes a0:"Re u > 0 " and 
+          a1:"Re v \<ge> 0 \<and> Im v = 0"
+        shows "Re (\<bar>u\<bar> * v) \<ge> 0  \<and> Im (\<bar>u\<bar> * v) = 0" 
+  using a0 a1
+  by (simp add: abs_complex_def)
+
+lemma vec_norm_Re_0:
+   "Re (vec_norm v) \<ge> 0 \<and> Im (vec_norm v) = 0"
+  unfolding vec_norm_def by auto
+
+lemma norm_complex_absolutely_homogenous:
+  assumes a1:"Re u > 0" 
+  shows "\<bar>u::complex\<bar> * vec_norm v = vec_norm( u \<cdot>\<^sub>v v)"
+proof-
+  have "\<bar>u\<bar> * vec_norm v = \<bar>u\<bar> * csqrt (v \<bullet>c v) "
+    unfolding vec_norm_def by auto
+  then have "(\<bar>u\<bar> * vec_norm v)^2  = (\<bar>u\<bar> * csqrt (v \<bullet>c v))^2"
+    by auto
+  also have "(\<bar>u\<bar> * csqrt (v \<bullet>c v))^2 = \<bar>u\<bar>^2 * (v \<bullet> (conjugate v))"
+    by (metis power2_csqrt power_mult_distrib)
+  also have "\<bar>u\<bar>^2 * (v \<bullet> (conjugate v)) = (u*(conjugate u)) * (v \<bullet> (conjugate v))"
+    using Complex.complex_norm_square by (simp add:  abs_complex_def) 
+  also have "(u*(conjugate u)) * (v \<bullet> (conjugate v)) = (u\<cdot>\<^sub>v v)  \<bullet> ((conjugate u)\<cdot>\<^sub>v(conjugate v))"
+    by auto
+  also have "(conjugate u::complex)\<cdot>\<^sub>v(conjugate v) = conjugate (u \<cdot>\<^sub>v v)"
+    by auto
+  finally have "csqrt ((\<bar>u\<bar> * vec_norm v)\<^sup>2) = csqrt (inner_prod (u \<cdot>\<^sub>v v) (u \<cdot>\<^sub>v v))"
+    by auto
+  also have "Re (\<bar>u\<bar> * vec_norm v) \<ge> 0 \<and> Im (\<bar>u\<bar> * vec_norm v) = 0" 
+    using Re_norm_u_gt_0_Im_v_0[OF a1] vec_norm_Re_0 by auto
+  then have "csqrt ((\<bar>u\<bar> * vec_norm v)\<^sup>2) = \<bar>u\<bar> * vec_norm v"
+    using csqrt_square
+    by (metis order_le_less)
+  finally show ?thesis
+    by (simp add: vec_norm_def)  
+qed
+
+
+lemma eq_vec_norm_q_empty:
+  assumes a0:"length (QStateM_list \<Q>'') = 1"
+  shows "vec_norm (QStateM_vector (QStateM_list \<Q>'' ! 0 \<cdot>\<^sub>Q \<Q>')) \<cdot>\<^sub>Q
    (inverse (QStateM_list \<Q>'' ! 0) \<cdot>\<^sub>Q \<Q>'') = 
   vec_norm (QStateM_vector \<Q>') \<cdot>\<^sub>Q \<Q>''"
-  sorry
+proof-
+  have f0:"Im (QStateM_list \<Q>'' ! 0) = 0 \<and> Re (QStateM_list \<Q>'' ! 0) > 0"
+    using a0 apply transfer by (auto;transfer;auto)
+  have f1:"Im (inverse (QStateM_list \<Q>'' ! 0)) = 0 \<and> Re (inverse (QStateM_list \<Q>'' ! 0)) > 0"
+    using f0 by auto
+  then have f2:"QStateM_vector (QStateM_list \<Q>'' ! 0 \<cdot>\<^sub>Q \<Q>') = 
+            QStateM_list \<Q>'' ! 0 \<cdot>\<^sub>v QStateM_vector \<Q>'"
+    using sca_mult_qstatem_var_qstate[OF f0, of \<Q>'] sca_mult_qstate_quantum[OF f0, of "qstate \<Q>'"]
+     apply auto
+    by (simp add: QStateM_vector.rep_eq qstate_def)
+  also have f3:"vec_norm (QStateM_list \<Q>'' ! 0 \<cdot>\<^sub>v QStateM_vector \<Q>') = 
+                 QStateM_list \<Q>'' ! 0 * vec_norm (QStateM_vector \<Q>')"  
+    using norm_complex_absolutely_homogenous[OF conjunct2[OF f0], of "QStateM_vector \<Q>'"] f0 
+    apply auto
+    by (simp add: abs_complex_def cmod_eq_Re complex_eq_iff) 
+  also have "QStateM_list \<Q>'' ! 0  \<cdot>\<^sub>Q (inverse (QStateM_list \<Q>'' ! 0) \<cdot>\<^sub>Q \<Q>'') = 
+            QStateM_list \<Q>'' ! 0 * (inverse (QStateM_list \<Q>'' ! 0))  \<cdot>\<^sub>Q \<Q>''"
+    using sca_mult_qstatem_assoc[OF f0 f1] by simp
+  then have "QStateM_list \<Q>'' ! 0 * vec_norm (QStateM_vector \<Q>') \<cdot>\<^sub>Q
+             (inverse (QStateM_list \<Q>'' ! 0) \<cdot>\<^sub>Q \<Q>'') = 
+            QStateM_list \<Q>'' ! 0 * vec_norm (QStateM_vector \<Q>') * (inverse (QStateM_list \<Q>'' ! 0))  \<cdot>\<^sub>Q \<Q>''"     
+    using f0
+    by (metis f1 sca_mult_qstate_def sca_mult_qstate_quantum sca_mult_qstate_vars 
+       sca_mult_qstatem_def sca_mult_qstatem_var_map sca_mult_qstatem_var_qstate smult_smult_assoc) 
+  finally show ?thesis
+    by (smt divide_complex_def f0 f2 f3 nonzero_mult_div_cancel_left zero_complex.simps(1))
+qed
+
 end
